Core/VCompFacts.v
@@ -9,10 +9,12 @@ From LHL.Core Require Import
 From LHL.Util Require Import
   Util.
 
-Lemma substIdImpl_is_id_l {M R} (p : Prog M R)
+(* Identity Laws for Program and Implementation Vertical Composition *)
+
+Lemma substIdImpl_is_id_l {E R} (p : Prog E R)
   : eutt ieq (substProg idImpl p) p.
 Proof.
-  enough (J : forall q p : Prog M R,
+  enough (J : forall q p : Prog E R,
              (q = substProg (fun _ m => Bind m Return) p \/
               q = NoOp (substProg (fun _ m => Bind m Return) p)) ->
              eutt ieq q p).
@@ -33,13 +35,13 @@ Proof.
     right. apply SELF. left. reflexivity.
 Defined.
 
-Lemma substIdImpl_is_id_r {E F} (impl : Impl E F)
+Lemma substIdImpl_is_id_r {E F} (M : Impl E F)
   {R} (f : F R)
-  : eutt ieq (substProg impl (idProg f)) (impl _ f).
+  : eutt ieq (substProg M (idProg f)) (M _ f).
 Proof.
   rewrite (frobProgId (substProg _ _)). cbn.
   apply eutt_NoOp_l.
-  remember (impl R f) as p eqn:E0. clear E0 f.
+  remember (M R f) as p eqn:E0. clear E0 f.
   revert p. pcofix SELF. intros p.
   pfold.
   destruct p;
@@ -51,17 +53,51 @@ Proof.
 Qed.
 
 Theorem idImpl_is_identity_l {E F Ret} : 
-    forall (impl : Impl E F) , 
-    euttImpl (Ret := Ret) ieq (idImpl |> impl) impl.
+    forall (M : Impl E F) , 
+    euttImpl (Ret := Ret) ieq (idImpl |> M) M.
 Proof.
   intros. unfold euttImpl. intros.
   apply substIdImpl_is_id_l.
 Qed.
 
 Theorem idImpl_is_identity_r {E F Ret} : 
-    forall (impl : Impl E F) , 
-    euttImpl (Ret := Ret) ieq (impl |> idImpl) impl.
+    forall (M : Impl E F) , 
+    euttImpl (Ret := Ret) ieq (M |> idImpl) M.
 Proof.
   intros. unfold euttImpl. intros.
   apply substIdImpl_is_id_r.
+Qed.
+
+(* Associativity *)
+
+Lemma substProg_assoc {E F G}
+      (f : Impl F G) (g : Impl E F)
+  : (ieq ==> eutt ieq)%isig
+      (fun _ (p : Prog G _) => substProg g (substProg f p))
+      (@substProg _ _ (fun _ (m : G _) =>
+                         substProg g (f _ m))).
+Proof.
+  intros ? e _ [].
+  enough (forall (p1 p2 : Prog E T),
+    subst_subst_bisim f g p1 p2 ->
+    eutt ieq p1 p2).
+  { apply H; constructor. }
+  clear. pcofix self; intros _ _ []; pfold.
+  all:
+    match goal with
+    | [ |- _ ?p1 ?p2 ] => rewrite (frobProgId p1), (frobProgId p2)
+    end;
+    match goal with
+    | [ p : Prog _ _ |- _ ] => destruct p; cbn
+    end; constructor.
+  all: try reflexivity.
+  all: right; apply self; constructor.
+Qed.
+
+Theorem implVComp_assoc {E F G H Ret} :
+  forall (MF : Impl E F) (MG : Impl F G) (MH : Impl G H),
+  euttImpl (Ret := Ret) ieq (MF |> (MG |> MH)) ((MF |> MG) |> MH).
+Proof.
+  intros. unfold euttImpl. intros.
+  apply substProg_assoc. reflexivity.
 Qed.
